README.md
@@ -7,6 +7,7 @@ Heya, I have been going through the exercises and trying to fill in all the
 - Chapter 3:
   - Section 3.1
   - Section 3.2
+  - Section 3.3
 
 
 # Lean formalization of _Analysis I_
